Protocol layer files for the Webserver example (wip)

ironfleet/src/Dafny/Distributed/Services/WS/WS.s.dfy
@@ -5,7 +5,7 @@ module WS__WS_s {
 import opened Native__Io_s
 
 datatype Request = Request(fileName:seq<char>)
-datatype Response = Response(r:seq<byte>) | Response404()
+datatype Response = ResponseValid(r:seq<byte>) | Response404()
 
 predicate SpecInit()
 {
@@ -16,6 +16,6 @@ predicate Get(fs:FileSystemState, req:Request, res:Response)
     requires fs != null;
 {
        fs != null
-    && (res == if fs.file_exists(req.fileName) then Response(fs.contents(req.fileName)) else Response404())
+    && (res == if fs.file_exists(req.fileName) then ResponseValid(fs.contents(req.fileName)) else Response404())
 }
 }
