ironfleet/src/Dafny/Distributed/Protocol/WS/Configuration.i.dfy
@@ -1,0 +1,18 @@
+include "Host.i.dfy"
+include "Parameters.i.dfy"
+
+module WS__Configuration_i {
+import opened WS__Host_i
+import opened Protocol_Parameters_i 
+
+datatype WSConfiguration = WSConfiguration(
+    clientIds:seq<NodeIdentity>,
+    hostIds:seq<NodeIdentity>,
+    rootIdentity:NodeIdentity,
+    params:Parameters)
+
+predicate WFSHTConfiguration(c:WSConfiguration)
+{
+       0 < |c.hostIds|
+}
+} 
