ironfleet/src/Dafny/Distributed/Protocol/WS/Environment.i.dfy
@@ -1,0 +1,20 @@
+include "Message.i.dfy"
+include "../../Common/Framework/Environment.s.dfy"
+
+module WS__Environment_i {
+import opened WS__Message_i
+import opened Environment_s
+
+type LWSEnvironment = LEnvironment<NodeIdentity, Message>
+type LWSPacket = LPacket<NodeIdentity, Message>
+type LWSIo = LIoOp<NodeIdentity, Message>
+
+function ConcatenateWSIos(s:seq<seq<LWSIo>>) : seq<LWSIo>
+{
+    if |s| == 0 then
+        []
+    else
+        s[0] + ConcatenateWSIos(s[1..])
+}
+
+}
