ironfleet/src/Dafny/Distributed/Protocol/WS/Host.i.dfy
@@ -1,0 +1,75 @@
+include "Parameters.i.dfy"
+include "Environment.i.dfy"
+include "Network.i.dfy"
+include "Message.i.dfy"
+include "../../Common/Collections/Sets.i.dfy"
+include "../../Common/Logic/Option.i.dfy"
+include "../../Services/WS/AbstractService.s.dfy"
+include "../Common/NodeIdentity.i.dfy"
+
+module WS__Host_i {
+import opened Protocol_Parameters_i 
+import opened WS__Environment_i
+import opened Collections__Sets_i
+import opened Logic__Option_i
+import opened AbstractServiceWS_s
+import opened Concrete_NodeIdentity_i
+import opened WS__Network_i
+import opened WS__Message_i
+
+datatype Constants = Constants(
+    hostIds:seq<NodeIdentity>,
+    params:Parameters)
+
+datatype Host = Host(
+    constants:Constants,
+    fs:FileSystemState,
+    me:NodeIdentity,
+    ghost receivedRequests:seq<AppRequest>
+    )
+
+function LWSPacketToPacket(lp:LWSPacket) : Packet
+{
+    Packet(lp.dst, lp.src, lp.msg)
+}
+
+function ExtractPacketsFromLWSPackets(seqPackets:seq<LWSPacket>) : set<Packet>
+    ensures forall p :: p in seqPackets <==> Packet(p.dst, p.src, p.msg) in ExtractPacketsFromLWSPackets(seqPackets)
+{
+    MapSeqToSet(seqPackets, LWSPacketToPacket)
+}
+
+predicate Host_Init(s:Host, id:NodeIdentity, hostIds:seq<NodeIdentity>, params:Parameters) {
+       s.constants == Constants(hostIds, params)
+    && s.me == id
+    && s.fs != null
+    && s.receivedRequests == []
+}
+
+predicate NextGetRequest_Reply(s:Host, s':Host, src:NodeIdentity, req:AppRequest, m:Message, out:set<Packet>)
+{ 
+        s.fs != null
+     && exists res :: Get(s.fs, Request(req.fileName), res)     
+     && m == GetResponse(res) 
+     && s'.receivedRequests == s.receivedRequests + [req]
+     && out == {Packet(src, s.me, m)}
+}
+
+predicate NextGetRequest(s:Host, s':Host, pkt:Packet, out:set<Packet>)
+{
+       pkt.msg.GetRequest?
+    && (exists m :: NextGetRequest_Reply(s, s', pkt.src, AppGetRequest(pkt.msg.req.fileName), m, out))
+}
+
+predicate Process_Message(s:Host, s':Host, recv:Packet, out:set<Packet>)
+{
+    NextGetRequest(s, s', recv, out)
+}
+
+predicate Host_Next(s:Host, s':Host, recv:Packet, out:set<Packet>)
+{
+       s'.constants == s.constants
+    && s'.me == s.me
+    && Process_Message(s, s', recv, out)
+} 
+}
