ironfleet/src/Dafny/Distributed/Protocol/WS/Message.i.dfy
@@ -1,0 +1,11 @@
+include "../Common/NodeIdentity.s.dfy"
+include "../../Services/WS/WS.s.dfy"
+
+module WS__Message_i {
+import opened Common__NodeIdentity_s
+import opened WS__WS_s
+
+datatype Message =
+      GetRequest(req:Request)
+    | GetResponse(resp:Response)
+} 
