ironfleet/src/Dafny/Distributed/Protocol/WS/Network.i.dfy
@@ -1,0 +1,29 @@
+include "Message.i.dfy"
+
+module WS__Network_i {
+import opened WS__Message_i
+
+datatype Packet = Packet(dst:NodeIdentity, src:NodeIdentity, msg:Message)
+
+type Network = set<Packet>
+
+predicate Network_Init(n:Network) {
+    n == {}
+}
+
+function PacketsTo(ps:set<Packet>, dst:NodeIdentity) : set<Packet>
+{
+    set p | p in ps && p.dst ==dst
+}
+
+predicate Network_Receive(n:Network, dst:NodeIdentity, recv:set<Packet>) {
+    recv == PacketsTo(n, dst)
+}
+
+predicate Network_Send(n:Network, n':Network, src:NodeIdentity, out:set<Packet>)
+{
+       (forall p :: p in out ==> p.src == src)  // Jay rewired this to have OutboundPackets
+    && n' == n + out
+}
+
+} 
